Proved map correctness for constraint closure

theory/shake.hs
@@ -1,0 +1,15 @@
+#!/usr/bin/env runhaskell
+
+import Development.Shake
+import Development.Shake.Util
+import Development.Shake.FilePath
+import Data.Maybe
+
+main = shakeArgs shakeOptions $ do  
+  want ["semantics.vo", "typecheck.vo", "lemmas.vo"]
+  "//*.vo" %> \out -> do
+    let source = out -<.> ".v"
+    deps <- cmd $ "coqdep " ++ source 
+    need $ fromMaybe [] $ lookup out $ parseMakefile $ fromStdout deps
+    cmd $ "coqc -I . " ++ source
+  phony "clean" $ removeFilesAfter "." ["//*.vo", "//*.glob"]
