theory/lemmas.v
@@ -1,0 +1,44 @@
+Require Import util syntax.  
+
+(* Read ω ∈* Ω as ω ∈ Ω* *)
+Reserved Notation " ω ∈* Ω " (at level 40).
+Inductive cclo (Ω : Ω) : ω → Prop := 
+  | trivial : ∀ ω, ω ∈ Ω → ω ∈* Ω
+  | sub_refl : ∀ r, subr r r ∈* Ω
+  | sub_trans : ∀ ri rj rk, subr ri rj ∈* Ω → subr rj rk ∈* Ω  → 
+                                  subr ri rk ∈* Ω 
+  | dis_sub : ∀ ri rj rk, subr ri rj ∈* Ω → disj rj rk ∈*  Ω → 
+                                  disj ri rk ∈* Ω
+  | dis_comm : ∀ ri rj, disj ri rj ∈* Ω → disj rj ri ∈* Ω 
+where " ω ∈* Ω " := (cclo Ω ω).
+
+Definition resp (M : M) (elem : Ω → ω → Prop) (Ω : Ω) :=
+  (∀ r1 r2, elem Ω (subr r1 r2) → lu r1 M ⊆ lu r2 M)
+                              ∧ 
+  (∀ r1 r2, elem Ω (disj r1 r2) → lu r1 M ∩ lu r2 M = [])
+.
+
+(* Read M ~* Ω as M ~ Ω* *)
+Notation " M ~ Ω " := (resp M (λ Ω ω, In ω Ω) Ω) (at level 40).
+Notation " M ~* Ω " := (resp M cclo Ω) (at level 40).
+
+Lemma resp_clos_sub : ∀ r1 r2 Ω (M:M), (∀ r1 r2, subr r1 r2 ∈ Ω → lu r1 M ⊆ lu r2 M) → 
+                                                 subr r1 r2 ∈* Ω → 
+																								lu r1 M ⊆ lu r2 M.
+intros. prep_induction H0. induction H0; intros; subst. apply H0. assumption.
+inversion H2. subst. clear H2. apply subset_refl. inversion H2. subst. clear H2.
+specialize (IHcclo2 _ _ _ H eq_refl).  specialize (IHcclo1 _ _ _ H eq_refl).
+apply (subset_trans _ _ _ IHcclo1 IHcclo2). inversion H2. inversion H2. Qed.
+
+Lemma resp_clos : ∀ M Ω, M ~ Ω ↔ M ~* Ω.
+intros. split; intros; split; intros; destruct H. apply resp_clos_sub with
+(Ω := Ω). assumption. assumption. prep_induction H0. induction
+H0; intros; subst. apply H1. assumption. inversion H3. subst. inversion H3.
+inversion H3. subst. clear H3.  specialize (IHcclo2 _ H H1 _ _ eq_refl). apply
+resp_clos_sub with (M:=M) in H0_. apply subset_intersection with (zs:=lu r2
+M) in H0_.  rewrite IHcclo2 in H0_. apply subset_nil_nil in H0_. assumption.
+assumption. inversion H3. subst. clear H3. specialize (IHcclo _ H H1 _ _ eq_refl). 
+apply subset_nil_nil. apply subset_trans with (ys:=lu r2 M ∩ lu r1 M). apply
+intersection_comm. rewrite IHcclo. apply subset_refl. apply H. apply trivial.
+assumption. apply H1. apply trivial. assumption. Qed.  
+
