theory/syntax.v
@@ -1,0 +1,85 @@
+Require Import util.  
+(* Syntax *)
+Definition r := nat. (* Logical region *)
+Definition l := nat. (* Location (pointer) *)
+Definition Color := nat.
+Definition set := list. (* We use lists for sets *)
+Definition ρ := set l. (* Physical region, which is a set of  *)
+Definition var := nat.
+Definition M := Map r ρ.
+Set Boolean Equality Schemes.
+
+(* Constraints *)
+Inductive ω := 
+  | subr : r → r → ω 
+  | disj : r → r → ω.
+Definition Ω := set ω.
+
+
+(* Privileges *)
+Inductive φ := 
+  | reads : r → φ 
+  | writes : r → φ 
+  | reduces : var → r → φ.
+Definition Φ := set φ.
+
+
+(* Coherence modes *)
+Inductive q := 
+  | atomic : r → q  
+  | simult : r → q.
+Definition Q := set q.
+
+(* Closures mode *) 
+
+Inductive T := 
+  | tbool 
+  | tint
+  | ttuple : list T → T
+  | pointer : T → list r → T
+  | coloring : r → T
+  | reg_rel : list r → T → Ω → T
+  | tfunction : list T → Φ → Q → T.
+
+Inductive v := 
+  | vbv : bool → v  
+  | viv : nat → v
+  | vtuple : list v → v
+  | vnull 
+  | vl : nat → v
+  | vcoloring : list (prod l nat) → v 
+  | vreg_rel : list ρ → v → v.
+
+Inductive e :=
+  | bv : bool → e
+  | iv : nat → e
+  | etuple : list e → e
+  | eindex : e → nat → e
+  | id : var → e
+  | new : T → r → e
+  | null : T → r → e
+  | isnull : e → e
+  | upr : e → list r → e
+  | downr : e → list r → e
+  | read : e → e 
+  | write : e → e → e
+  | reduce : var → e → e
+  | newcolor : r → e
+  | color : e → e → e → e
+  | add : e → e → e
+  | lt : e → e → e
+  | elet : var → T → e → e → e
+  | eif : e → e → e → e
+  | call : var → list r → list e → e
+  | partition : r → e → list r → e → e
+  | pack : e → T → list r → e
+  | unpack : e → var → T → list r → e → e.
+
+(* Inductive definition for what functions are defined, default to any *)
+Inductive function : var → list r → list var → list T → Φ → Q → T → e → Prop := 
+  | mkfunction : ∀ id rs xs Ts T Phi Q e, function id rs xs Ts T Phi Q e.
+
+Inductive memop := 
+  | mread : l → memop
+  | mwrite : l → v → memop
+  | mreduce : l → var → v → memop.
