theory/typecheck.v
@@ -1,0 +1,41 @@
+Require Import util syntax.
+Require Import Strings.String.
+Open Scope type_scope.
+Open Scope string_scope.
+
+(*
+Inductive T := 
+  | tbool 
+  | tint
+  | ttuple : list T → T
+  | pointer : T → list r → T
+  | coloring : r → T
+  | reg_rel : list r → T → Ω → T
+  | tfunction : list T → Φ → Q → T.
+*)
+
+Definition Γ := Map var T.
+
+Fixpoint typecheck (env : (Γ * Φ * Ω)) (e : e) : T + string := let '(Γ, Φ, Ω) := env in 
+  match e with
+  | read e => match typecheck env e with 
+    | inl (pointer t rs) => if forallb (λ r, existsb (φ_beq (reads r)) Φ) rs
+        then inl t
+        else inr "don't have read permission"
+    | inl _ => inr "expected pointer type"
+    | inr x => inr x
+    end
+  | write e₁ e₂ => match typecheck env e₁ with
+    | inl (pointer t rs) => if forallb (λ r, existsb (φ_beq (writes r)) Φ) rs
+        then match typecheck env e₂ with
+          | inl t' => if T_beq t t' then inl t else inr "mismatched types for write"
+          | inr e => inr e
+          end
+        else inr "don't have write permission"
+    | inl _ => inr "expected pointer type"
+    | inr x => inr x
+    end
+  | _ => inr "unimplemented"
+  end.
+  
+Reserved Notation " xs ⊢ e :: T " (at level 50). 
