theory/util.v
@@ -1,0 +1,108 @@
+Require Export Unicode.Utf8.
+Require Export JRWTactics.
+Require Export List Init.Datatypes.
+Export ListNotations.
+Open Scope program_scope.
+
+Require Export EqNat Arith.Peano_dec Program.Basics.
+
+Definition all := fold_right andb true.
+
+Fixpoint zip {a b} (xs : list a) (ys : list b) : list (prod a b) := 
+  match xs, ys with
+  | [], _ => []
+  | _, [] => []
+  | x::xs, y::ys => (x,y)::zip xs ys
+  end.
+
+Fixpoint contains {a} (eq : a → a → bool) (y : a) (xs : list a) := 
+  match xs with 
+  | [] => false
+  | x::xs => if eq x y then true else contains eq y xs
+  end.
+
+
+Fixpoint groupBy {a} (f : a → a → bool) (xs : list a) := match xs with  
+  | [] => []
+  | x::xs => (x::filter (f x) xs) :: filter (negb ∘ contains f x) (groupBy f xs)
+  end.
+  
+Definition Map a b := list (prod a b).
+
+Definition lookup {a} (x:nat) (l:Map nat a) : option a := 
+  match find (λ p, beq_nat x (fst p)) l with 
+    | None => None
+    | Some (k,v) => Some v
+  end.
+
+Notation " x ∈ y " := (In x y) (at level 30).
+Notation " x ∉ y " := (¬ In x y) (at level 30).
+
+Definition subset {a} xs ys := ∀ x:a, In x xs → In x ys.
+Notation " x ⊆ y " := (subset x y) (at level 50).
+
+Lemma subset_nil_nil {a} : ∀ xs:list a, xs ⊆ [] → xs = [].
+intros. unfold subset in H. simpl in H. destruct xs. auto. assert False.
+apply H with (x:=a0). simpl. apply or_introl. auto. inversion H0. Qed.
+
+Lemma subset_refl {a} : ∀ xs:list a, subset xs xs. intros. unfold subset;
+intros. assumption. Qed. 
+
+Lemma subset_trans {a} : ∀ xs ys zs : list a, xs ⊆ ys → ys ⊆ zs → xs ⊆ zs.
+intros. unfold subset. intros. apply H in H1. apply H0. assumption. Qed. 
+
+Lemma contains_beq_nat_in : ∀ x xs, contains beq_nat x xs = true ↔ x ∈ xs.
+intros; split; intros. induction xs. simpl in H. inversion H. simpl. simpl in
+H. destruct (PeanoNat.Nat.eqb a x) eqn:ax. apply beq_nat_true in ax. subst.
+apply or_introl.  reflexivity. apply or_intror. apply IHxs. assumption.
+induction xs. inversion H. destruct H . subst. simpl. rewrite <- beq_nat_refl.
+reflexivity. apply IHxs in H. simpl. rewrite H. destruct (beq_nat a x); auto.
+Qed.  
+
+Lemma contains_beq_nat_not_in : ∀ x xs, contains beq_nat x xs = false ↔ x ∉ xs.
+intros; split; intros. induction xs. auto. simpl in H. destruct
+(PeanoNat.Nat.eqb a x) eqn:ax. inversion H. apply beq_nat_false in ax. unfold
+not. intros. destruct H0. subst. apply ax. reflexivity. apply IHxs in H. apply
+H. assumption. induction xs; intros. auto. simpl. destruct (beq_nat a x) eqn:ax.
+simpl in H.  assert False. apply H. apply or_introl. apply beq_nat_true in ax.
+assumption. inversion H0. apply IHxs. unfold not. intros. unfold not in H.
+apply H. simpl. apply or_intror. assumption. Qed.
+
+Fixpoint intersection (xs ys : list nat) : list nat := match xs with
+  | [] => []
+  | x::xs => (if contains beq_nat x ys then cons x else id) (intersection xs ys)
+  end.
+
+Notation " x ∩ y " := (intersection x y) (at level 50).
+
+Lemma intersection_in : ∀ x xs ys, x ∈ (xs ∩ ys) ↔ x ∈ xs ∧ x ∈ ys.
+intros. split; intros. induction xs; intros. inversion
+H. simpl in H.  destruct (contains PeanoNat.Nat.eqb a ys) eqn:cays. simpl in H. destruct H. subst. 
+rewrite contains_beq_nat_in in cays. split. simpl. apply or_introl. reflexivity. assumption. apply IHxs in H. 
+destruct H. split. apply or_intror. assumption. assumption. rewrite contains_beq_nat_not_in in cays. apply IHxs in H. 
+destruct H. split. apply or_intror. assumption. assumption. induction xs. simpl. destruct H. inversion H. simpl. simpl. 
+destruct (contains beq_nat a ys) eqn:cays. simpl. destruct H. rewrite contains_beq_nat_in in cays. simpl in H. destruct H. 
+subst. apply or_introl. reflexivity. apply or_intror. apply IHxs. split; assumption. apply IHxs. destruct H. 
+rewrite contains_beq_nat_not_in in cays. destruct H. subst. apply cays in H0. inversion H0. split; assumption. Qed. 
+
+Definition seteq {a} (xs ys : list a) := subset xs ys /\ subset ys xs. 
+
+Lemma intersection_comm : forall xs ys, subset (intersection xs ys) (intersection ys xs).
+intros. unfold subset; intros. rewrite intersection_in. rewrite intersection_in in H. 
+destruct H. split; auto. Qed. 
+
+Lemma subset_intersection : ∀ xs ys zs, xs ⊆ ys → (xs ∩ zs) ⊆ (ys ∩ zs).
+intros. unfold subset. intros. rewrite intersection_in. rewrite intersection_in in H0. 
+destruct H0. apply H in H0. split; auto. Qed.
+
+Fixpoint inits {a} (xs : list a) : list (list a) := match xs with
+  | [] => []
+  | x::xs => [x] :: map (cons x) (inits xs)
+  end.
+
+Definition lu {a} (x:nat) (l:Map nat (list a)) : list a := 
+  match lookup x l with 
+    | None => []
+    | Some l => l
+  end.
+
